Refactoring separation-logic predicates so that forward(), do_scan(), etc. do not need the entire thread_info, but can take just the heap and the root set.  This allows proofs of those functions to be agnostic regarding how the roots are found (in the stack, in the args[] array, etc.).

CertiGC/GCGraph.v
@@ -536,13 +536,13 @@ Definition generation_space_compatible (g: LGraph)
 
 Local Close Scope Z_scope.
 
-Definition graph_thread_info_compatible (g: LGraph) (ti: thread_info): Prop :=
+Definition graph_heap_compatible (g: LGraph) (h: heap): Prop :=
   Forall (generation_space_compatible g)
          (combine (combine (nat_inc_list (length g.(glabel).(g_gen)))
-                           g.(glabel).(g_gen)) ti.(ti_heap).(spaces)) /\
+                           g.(glabel).(g_gen)) h.(spaces)) /\
   Forall (eq nullval)
-         (skipn (length g.(glabel).(g_gen)) (map space_start ti.(ti_heap).(spaces))) /\
-  length g.(glabel).(g_gen) <= length ti.(ti_heap).(spaces).
+         (skipn (length g.(glabel).(g_gen)) (map space_start h.(spaces))) /\
+  length g.(glabel).(g_gen) <= length h.(spaces).
 
 Definition vertex_offset (g: LGraph) (v: VType): Z :=
   previous_vertices_size g (vgeneration v) (vindex v) + 1.
@@ -648,14 +648,24 @@ Definition copy_compatible (g: LGraph): Prop :=
             graph_has_v g (vlabel g v).(copied_vertex) /\
             vgeneration v <> vgeneration (vlabel g v).(copied_vertex).
 
+Definition super_compatible' (g: LGraph) (h: heap) (frames: list frame) (r: roots_t) (out: outlier_t) : Prop := 
+  graph_heap_compatible g h /\
+  frames_compatible g frames r /\
+  roots_compatible g out r /\
+  outlier_compatible g out.
+
 Definition super_compatible
   (g_ti_r: LGraph * thread_info * roots_t) (out: outlier_t) : Prop :=
+   super_compatible' (fst (fst g_ti_r)) (ti_heap (snd (fst g_ti_r))) (ti_frames (snd (fst g_ti_r))) (snd g_ti_r) out.
+
+(*
   let (g_ti, r) := g_ti_r in
   let (g, ti) := g_ti in
   graph_thread_info_compatible g ti /\
   frames_compatible g (ti_frames ti) r /\
   roots_compatible g out r /\
   outlier_compatible g out.
+*)
 
 Definition reset_gen_info (gi: generation_info) : generation_info :=
   Build_generation_info (start_address gi) O (generation_sh gi) (start_isptr gi)
@@ -826,11 +836,11 @@ Definition reset_nth_heap_thread_info (n: nat) (ti: thread_info) : thread_info :
   Build_thread_info (ti_heap_p ti) (reset_nth_heap n (ti_heap ti))
                     (ti_args ti) (arg_size ti) (ti_frames ti) (ti_nalloc ti).
 
-Lemma reset_thread_info_overflow: forall n ti,
-    length (spaces (ti_heap ti)) <= n -> reset_nth_heap_thread_info n ti = ti.
+
+Lemma reset_heap_overflow: forall n h,
+    length (spaces h) <= n -> reset_nth_heap n h = h.
 Proof.
-  intros. unfold reset_nth_heap_thread_info. destruct ti. f_equal.
-  simpl. unfold reset_nth_heap. destruct ti_heap0. simpl in *.
+  intros. unfold reset_nth_heap.  destruct h. simpl in *.
   assert (spaces0 = reset_nth_space n spaces0) by
       (rewrite reset_nth_space_overflow; [reflexivity | assumption]).
   apply EqdepFacts.f_eq_dep_non_dep, EqdepFacts.eq_dep1_dep.
@@ -1677,11 +1687,11 @@ Inductive forward_roots_loop (from to: nat):
 Definition forward_roots_relation from to roots1 g1 roots2 g2 :=
   forward_roots_loop from to (nat_inc_list (length roots1)) roots1 g1 roots2 g2.
 
-Definition nth_space (t_info: thread_info) (n: nat): space :=
-  nth n t_info.(ti_heap).(spaces) null_space.
+Definition nth_space (h: heap) (n: nat): space :=
+  nth n h.(spaces) null_space.
 
-Lemma nth_space_Znth: forall t n,
-    nth_space t n = Znth (Z.of_nat n) (spaces (ti_heap t)).
+Lemma nth_space_Znth: forall h n,
+    nth_space h n = Znth (Z.of_nat n) (spaces h).
 Proof.
   intros. unfold nth_space, Znth. rewrite if_false. 2: lia.
   rewrite Nat2Z.id. reflexivity.
@@ -1689,32 +1699,32 @@ Qed.
 
 Definition gen_size t_info n := total_space (nth_space t_info n).
 
-Lemma gsc_iff: forall (g: LGraph) t_info,
-    length (g_gen (glabel g)) <= length (spaces (ti_heap t_info)) ->
+Lemma gsc_iff: forall (g: LGraph) h,
+    length (g_gen (glabel g)) <= length (spaces h) ->
     Forall (generation_space_compatible g)
            (combine (combine (nat_inc_list (length (g_gen (glabel g))))
-                             (g_gen (glabel g))) (spaces (ti_heap t_info))) <->
+                             (g_gen (glabel g))) (spaces h)) <->
     forall gen,
       graph_has_gen g gen ->
-      generation_space_compatible g (gen, nth_gen g gen, nth_space t_info gen).
+      generation_space_compatible g (gen, nth_gen g gen, nth_space h gen).
 Proof.
   intros. rewrite Forall_forall. remember (g_gen (glabel g)).
-  remember (nat_inc_list (length l)). remember (spaces (ti_heap t_info)).
+  remember (nat_inc_list (length l)). remember (spaces h).
   assert (length (combine l0 l) = length l) by
       (subst; rewrite combine_length, nat_inc_list_length, Nat.min_id; reflexivity).
   assert (length (combine (combine l0 l) l1) = length l) by
       (rewrite combine_length, H0, min_l by assumption; reflexivity).
   cut (forall x, In x (combine (combine l0 l) l1) <->
                     exists gen, graph_has_gen g gen /\
-                                x = (gen, nth_gen g gen, nth_space t_info gen)).
+                                x = (gen, nth_gen g gen, nth_space h gen)).
   - intros. split; intros.
-    + apply H3. rewrite H2. exists gen. intuition.
-    + rewrite H2 in H4. destruct H4 as [gen [? ?]]. subst x. apply H3. assumption.
+    + apply H3. rewrite H2. exists gen. subst l1; intuition.
+    + rewrite H2 in H4. destruct H4 as [gen [? ?]]. subst l1 x. apply H3. assumption.
   - intros.
     assert (forall gen,
                graph_has_gen g gen ->
                nth gen (combine (combine l0 l) l1) (0, null_info, null_space) =
-               (gen, nth_gen g gen, nth_space t_info gen)). {
+               (gen, nth_gen g gen, nth_space h gen)). {
       intros. red in H2. rewrite <- Heql in H2.
       rewrite combine_nth_lt; [|rewrite H0; lia | lia].
       rewrite combine_nth by (subst l0; rewrite nat_inc_list_length; reflexivity).
@@ -1730,11 +1740,11 @@ Proof.
 Qed.
 
 Lemma gt_gs_compatible:
-  forall (g: LGraph) (t_info: thread_info),
-    graph_thread_info_compatible g t_info ->
+  forall (g: LGraph) (h: heap),
+    graph_heap_compatible g h ->
     forall gen,
       graph_has_gen g gen ->
-      generation_space_compatible g (gen, nth_gen g gen, nth_space t_info gen).
+      generation_space_compatible g (gen, nth_gen g gen, nth_space h gen).
 Proof.
   intros. destruct H as [? [_ ?]]. rewrite gsc_iff in H by assumption.
   apply H. assumption.
@@ -1768,9 +1778,8 @@ Qed.
 Local Open Scope Z_scope.
 
 Definition forward_roots_compatible
-           (from to: nat) (g: LGraph) (ti : thread_info): Prop :=
-  (nth_space ti from).(used_space) <= (nth_space ti to).(total_space) -
-                                      (nth_space ti to).(used_space).
+           (from to: nat) (g: LGraph) (h: heap): Prop :=
+  (nth_space h from).(used_space) <= (nth_space h to).(total_space) - (nth_space h to).(used_space).
 
 Lemma vo_lt_gs: forall g v,
     gen_has_index g (vgeneration v) (vindex v) ->
@@ -1787,18 +1796,18 @@ Qed.
 Definition v_in_range (v: val) (start: val) (n: Z): Prop :=
   exists i, 0 <= i < n /\ v = offset_val i start.
 
-Lemma graph_thread_v_in_range: forall g t_info v,
-    graph_thread_info_compatible g t_info -> graph_has_v g v ->
+Lemma graph_thread_v_in_range: forall g h v,
+    graph_heap_compatible g h -> graph_has_v g v ->
     v_in_range (vertex_address g v) (gen_start g (vgeneration v))
-               (WORD_SIZE * gen_size t_info (vgeneration v)).
+               (WORD_SIZE * gen_size h (vgeneration v)).
 Proof.
   intros. red. unfold vertex_address. exists (WORD_SIZE * vertex_offset g v).
   split. 2: reflexivity. unfold gen_size. destruct H0. remember (vgeneration v). split.
   - unfold vertex_offset. unfold WORD_SIZE.
     pose proof (pvs_ge_zero g (vgeneration v) (vindex v)). rep_lia.
   - unfold WORD_SIZE. apply Zmult_lt_compat_l. 1: rep_lia.
-    apply Z.lt_le_trans with (used_space (nth_space t_info n)).
-    2: apply (proj2 (space_order (nth_space t_info n))).
+    apply Z.lt_le_trans with (used_space (nth_space h n)).
+    2: apply (proj2 (space_order (nth_space h n))).
     destruct (gt_gs_compatible _ _ H _ H0) as [? [? ?]].
     rewrite <- H4, Heqn. apply vo_lt_gs. subst n. assumption.
 Qed.
@@ -1858,8 +1867,8 @@ Proof.
       [intros; apply Z.le_lteq; left; apply vsa_mono | apply vsa_comm | apply H1].
 Qed.
 
-Definition rest_gen_size (t_info: thread_info) (gen: nat): Z :=
-  total_space (nth_space t_info gen) - used_space (nth_space t_info gen).
+Definition rest_gen_size (h: heap) (gen: nat): Z :=
+  total_space (nth_space h gen) - used_space (nth_space h gen).
 
 Definition enough_space_to_copy g t_info from to: Prop :=
   unmarked_gen_size g from <= rest_gen_size t_info to.
@@ -1922,10 +1931,10 @@ Definition cut_thread_info (t: thread_info) (i s: Z)
   Build_thread_info (ti_heap_p t) (cut_heap (ti_heap t) i s H1 H2) (ti_args t)
                     (arg_size t) (ti_frames t) (ti_nalloc t).
 
-Lemma cti_eq: forall t i s1 s2 (H1: 0 <= i < Zlength (spaces (ti_heap t)))
-                     (Hs1: has_space (Znth i (spaces (ti_heap t))) s1)
-                     (Hs2: has_space (Znth i (spaces (ti_heap t))) s2),
-    s1 = s2 -> cut_thread_info t i s1 H1 Hs1 = cut_thread_info t i s2 H1 Hs2.
+Lemma cti_eq: forall h i s1 s2 (H1: 0 <= i < Zlength (spaces h))
+                     (Hs1: has_space (Znth i (spaces h)) s1)
+                     (Hs2: has_space (Znth i (spaces h)) s2),
+    s1 = s2 -> cut_heap h i s1 H1 Hs1 = cut_heap h i s2 H1 Hs2.
 Proof.
   intros. unfold cut_thread_info. f_equal. subst s1. f_equal. apply proof_irr.
 Qed.
@@ -2511,17 +2520,10 @@ Proof. intros. apply lmc_outlier_compatible, lacv_outlier_compatible; assumption
 
 Local Open Scope Z_scope.
 
-Lemma utia_estc: forall g t_info from to index v,
-    enough_space_to_copy g t_info from to ->
-    enough_space_to_copy g 
-    (update_thread_info_frames
-         t_info 
-         (update_frames (ti_frames t_info)
-            (upd_Znth index (frames2roots (ti_frames t_info)) v)))
-   from to.
-Proof.
-  unfold enough_space_to_copy. intros. unfold rest_gen_size, nth_space in *.
-  apply H.
+Lemma utia_estc: forall g t_info from to frames,
+    enough_space_to_copy g t_info.(ti_heap) from to ->
+    enough_space_to_copy g (update_thread_info_frames t_info frames).(ti_heap) from to.
+Proof. intros. apply H.
 Qed.
 
 Lemma lacv_unmarked_gen_size: forall g v to from,
@@ -2590,26 +2592,25 @@ Proof.
 Qed.
 
 Lemma cti_rest_gen_size:
-  forall t_info to s
-         (Hi : 0 <= Z.of_nat to < Zlength (spaces (ti_heap t_info)))
-         (Hh : has_space (Znth (Z.of_nat to) (spaces (ti_heap t_info))) s),
-  rest_gen_size t_info to =
-  rest_gen_size (cut_thread_info t_info (Z.of_nat to) s Hi Hh) to + s.
+  forall h to s
+         (Hi : 0 <= Z.of_nat to < Zlength (spaces h))
+         (Hh : has_space (Znth (Z.of_nat to) (spaces h)) s),
+  rest_gen_size h to =
+  rest_gen_size (cut_heap h (Z.of_nat to) s Hi Hh) to + s.
 Proof.
   intros. unfold rest_gen_size. rewrite !nth_space_Znth. unfold cut_thread_info. simpl.
   rewrite upd_Znth_same by assumption. simpl. lia.
 Qed.
 
 Lemma lmc_estc:
-  forall (g : LGraph) (t_info : thread_info) (v v': VType) (to : nat)
-         (Hi : 0 <= Z.of_nat to < Zlength (spaces (ti_heap t_info))),
-    enough_space_to_copy g t_info (vgeneration v) to ->
+  forall (g : LGraph) (h : heap) (v v': VType) (to : nat)
+         (Hi : 0 <= Z.of_nat to < Zlength (spaces h)),
+    enough_space_to_copy g h (vgeneration v) to ->
     graph_has_v g v -> raw_mark (vlabel g v) = false ->
     forall
-      Hh : has_space (Znth (Z.of_nat to) (spaces (ti_heap t_info))) (vertex_size g v),
+      Hh : has_space (Znth (Z.of_nat to) (spaces h)) (vertex_size g v),
       enough_space_to_copy (lgraph_mark_copied g v v')
-                           (cut_thread_info
-                              t_info (Z.of_nat to) (vertex_size g v) Hi Hh)
+                           (cut_heap h (Z.of_nat to) (vertex_size g v) Hi Hh)
                            (vgeneration v) to.
 Proof.
   unfold enough_space_to_copy. intros.
@@ -2618,14 +2619,14 @@ Proof.
 Qed.
 
 Lemma forward_estc_unchanged: forall
-    g t_info v to
-    (Hi : 0 <= Z.of_nat to < Zlength (spaces (ti_heap t_info)))
-    (Hh : has_space (Znth (Z.of_nat to) (spaces (ti_heap t_info))) (vertex_size g v)),
+    g h v to
+    (Hi : 0 <= Z.of_nat to < Zlength (spaces h))
+    (Hh : has_space (Znth (Z.of_nat to) (spaces h)) (vertex_size g v)),
     vgeneration v <> to -> graph_has_gen g to ->
     graph_has_v g v -> raw_mark (vlabel g v) = false ->
-    enough_space_to_copy g t_info (vgeneration v) to ->
+    enough_space_to_copy g h (vgeneration v) to ->
     enough_space_to_copy (lgraph_copy_v g v to)
-         (cut_thread_info t_info (Z.of_nat to) (vertex_size g v) Hi Hh)
+         (cut_heap h (Z.of_nat to) (vertex_size g v) Hi Hh)
       (vgeneration v) to.
 Proof.
   intros. unfold lgraph_copy_v.
@@ -2636,8 +2637,8 @@ Proof.
     inversion H4. apply H. assumption. }
   remember (lgraph_add_copied_v g v to) as g'.
   pose proof Hh as Hh'. rewrite H4 in Hh'.
-  replace (cut_thread_info t_info (Z.of_nat to) (vertex_size g v) Hi Hh) with
-      (cut_thread_info t_info (Z.of_nat to) (vertex_size g' v) Hi Hh') by
+  replace (cut_heap h (Z.of_nat to) (vertex_size g v) Hi Hh) with
+      (cut_heap h (Z.of_nat to) (vertex_size g' v) Hi Hh') by
       (apply cti_eq; symmetry; assumption).
   apply lmc_estc.
   - assumption.
@@ -2646,39 +2647,30 @@ Proof.
 Qed.
 
 Lemma forward_estc: forall
-    g t_info v to index uv
-    (Hi : 0 <= Z.of_nat to < Zlength (spaces (ti_heap t_info)))
-    (Hh : has_space (Znth (Z.of_nat to) (spaces (ti_heap t_info))) (vertex_size g v))
-    (*Hm : 0 <= index < MAX_ARGS*),
+    g h v to
+    (Hi : 0 <= Z.of_nat to < Zlength (spaces h))
+    (Hh : has_space (Znth (Z.of_nat to) (spaces h)) (vertex_size g v)),
     vgeneration v <> to -> graph_has_gen g to ->
     graph_has_v g v -> raw_mark (vlabel g v) = false ->
-    enough_space_to_copy g t_info (vgeneration v) to ->
+    enough_space_to_copy g h (vgeneration v) to ->
     enough_space_to_copy
       (lgraph_copy_v g v to)
-      (update_thread_info_frames
-         (cut_thread_info t_info (Z.of_nat to) (vertex_size g v) Hi Hh)
-         (update_frames (ti_frames t_info)
-            (upd_Znth index (frames2roots (ti_frames t_info)) uv)))
+         (cut_heap h (Z.of_nat to) (vertex_size g v) Hi Hh)
       (vgeneration v) to.
 Proof.
   intros. 
-  change (ti_frames t_info) with (ti_frames (cut_thread_info t_info (Z.of_nat to) (vertex_size g v) Hi Hh)).
-  apply utia_estc.
-  apply forward_estc_unchanged; assumption.
+  apply forward_estc_unchanged; assumption.  (* REDUNDANT? *)
 Qed.
 
 Lemma lcv_forward_condition: forall
-    g t_info v to index uv
-    (Hi : 0 <= Z.of_nat to < Zlength (spaces (ti_heap t_info)))
-    (Hh : has_space (Znth (Z.of_nat to) (spaces (ti_heap t_info))) (vertex_size g v)),
+    g h v to
+    (Hi : 0 <= Z.of_nat to < Zlength (spaces h))
+    (Hh : has_space (Znth (Z.of_nat to) (spaces h)) (vertex_size g v)),
     vgeneration v <> to -> graph_has_v g v -> raw_mark (vlabel g v) = false ->
-    forward_condition g t_info (vgeneration v) to ->
+    forward_condition g h (vgeneration v) to ->
     forward_condition
       (lgraph_copy_v g v to)
-     (update_thread_info_frames
-        (cut_thread_info t_info (Z.of_nat to) (vertex_size g v) Hi Hh)
-        (update_frames (ti_frames t_info)
-           (upd_Znth index (frames2roots (ti_frames t_info)) uv)))
+        (cut_heap h (Z.of_nat to) (vertex_size g v) Hi Hh)
       (vgeneration v) to.
 Proof.
   intros. destruct H2 as [? [? [? [? ?]]]]. split; [|split; [|split; [|split]]].
@@ -2689,14 +2681,14 @@ Proof.
   - apply lcv_no_dangling_dst; assumption.
 Qed.
 
-Lemma lcv_forward_condition_unchanged: forall
-    g t_info v to
-    (Hi : 0 <= Z.of_nat to < Zlength (spaces (ti_heap t_info)))
-    (Hh : has_space (Znth (Z.of_nat to) (spaces (ti_heap t_info))) (vertex_size g v)),
+Lemma lcv_forward_condition_unchanged: forall (* REDUNDANT WITH PREVIOUS LEMMA? *)
+    g h v to
+    (Hi : 0 <= Z.of_nat to < Zlength (spaces h))
+    (Hh : has_space (Znth (Z.of_nat to) (spaces h)) (vertex_size g v)),
     vgeneration v <> to -> graph_has_v g v -> raw_mark (vlabel g v) = false ->
-    forward_condition g t_info (vgeneration v) to ->
+    forward_condition g h (vgeneration v) to ->
     forward_condition (lgraph_copy_v g v to)
-         (cut_thread_info t_info (Z.of_nat to) (vertex_size g v) Hi Hh)
+         (cut_heap h (Z.of_nat to) (vertex_size g v) Hi Hh)
       (vgeneration v) to.
 Proof.
   intros. destruct H2 as [? [? [? [? ?]]]]. split; [|split; [|split; [|split]]].
@@ -2784,14 +2776,11 @@ Proof.
 Qed.
 
 Lemma lcv_frames_compatible_unchanged: forall
-    g t_info roots v to i s
-    (Hi : 0 <= i < Zlength (spaces (ti_heap t_info)))
-    (Hh : has_space (Znth i (spaces (ti_heap t_info))) s),
+    g frames roots v to,
     graph_has_gen g to ->
     roots_graph_compatible roots g ->
-    frames_compatible g (ti_frames t_info) roots ->
-    frames_compatible (lgraph_copy_v g v to)
-         (ti_frames (cut_thread_info t_info i s Hi Hh)) roots.
+    frames_compatible g frames roots ->
+    frames_compatible (lgraph_copy_v g v to) frames roots.
 Proof.
  intros.
  unfold cut_thread_info, frames_compatible in *; simpl in *.
@@ -2864,22 +2853,22 @@ Qed.
 
 
 Lemma lcv_frames_compatible: forall
-    g t_info roots z v to i s
-    (Hi : 0 <= i < Zlength (spaces (ti_heap t_info)))
-    (Hh : has_space (Znth i (spaces (ti_heap t_info))) s)
+    g h frames roots z v to i s
+    (Hi : 0 <= i < Zlength (spaces h))
+    (Hh : has_space (Znth i (spaces h)) s)
     (Hm : 0 <= z < Zlength roots),
     graph_has_gen g to -> roots_graph_compatible roots g ->
-    frames_compatible g (ti_frames t_info) roots ->
+    frames_compatible g frames roots ->
     frames_compatible 
       (lgraph_copy_v g v to)
-      (update_frames (ti_frames t_info) 
-        (upd_Znth z (frames2roots (ti_frames t_info)) 
+      (update_frames frames 
+        (upd_Znth z (frames2roots frames) 
           (vertex_address g (new_copied_v g to))))
       (upd_Znth z roots (inr (new_copied_v g to))).
 Proof.
   intros. rewrite <- (lcv_vertex_address_new g v to H).
-  apply (lcv_frames_compatible_unchanged g t_info roots v to i s Hi Hh) in H1; try assumption.
   apply upd_frames_compatible; auto.
+  apply lcv_frames_compatible_unchanged; assumption. 
 Qed.
 
 (*
@@ -2964,21 +2953,20 @@ Proof.
 Qed.
 
 Lemma lcv_graph_thread_info_compatible: forall
-    g t_info v to
-    (Hi : 0 <= Z.of_nat to < Zlength (spaces (ti_heap t_info)))
-    (Hh : has_space (Znth (Z.of_nat to) (spaces (ti_heap t_info))) (vertex_size g v)),
+    g h v to
+    (Hi : 0 <= Z.of_nat to < Zlength (spaces h))
+    (Hh : has_space (Znth (Z.of_nat to) (spaces h)) (vertex_size g v)),
     graph_has_gen g to ->
-    graph_thread_info_compatible g t_info ->
-    graph_thread_info_compatible (lgraph_copy_v g v to)
-      (cut_thread_info t_info (Z.of_nat to) (vertex_size g v)
-                       Hi Hh).
+    graph_heap_compatible g h ->
+    graph_heap_compatible (lgraph_copy_v g v to)
+      (cut_heap h (Z.of_nat to) (vertex_size g v) Hi Hh).
 Proof.
-  unfold graph_thread_info_compatible. intros. destruct H0 as [? [? ?]].
-  assert (map space_start (spaces (ti_heap t_info)) =
+  unfold graph_heap_compatible. intros. destruct H0 as [? [? ?]].
+  assert (map space_start (spaces h) =
           map space_start
-              (upd_Znth (Z.of_nat to) (spaces (ti_heap t_info))
+              (upd_Znth (Z.of_nat to) (spaces h)
                         (cut_space
-                           (Znth (Z.of_nat to) (spaces (ti_heap t_info)))
+                           (Znth (Z.of_nat to) (spaces h))
                            (vertex_size g v) Hh))). {
     rewrite <- upd_Znth_map. simpl. rewrite <- Znth_map by assumption.
     rewrite upd_Znth_unchanged; [reflexivity | rewrite Zlength_map; assumption]. }
@@ -2992,18 +2980,18 @@ Proof.
         -- subst gen. rewrite cvmgil_eq; simpl; assumption.
         -- rewrite cvmgil_not_eq; assumption.
       * assert (map space_sh
-                    (upd_Znth (Z.of_nat to) (spaces (ti_heap t_info))
+                    (upd_Znth (Z.of_nat to) (spaces h)
                               (cut_space
-                                 (Znth (Z.of_nat to) (spaces (ti_heap t_info)))
+                                 (Znth (Z.of_nat to) (spaces h))
                                  (vertex_size g v) Hh)) =
-                map space_sh (spaces (ti_heap t_info))). {
+                map space_sh (spaces h)). {
           rewrite <- upd_Znth_map. simpl. rewrite <- Znth_map by assumption.
           rewrite upd_Znth_unchanged; [reflexivity|rewrite Zlength_map; assumption]. }
         rewrite <- map_nth, H7, map_nth. clear -H5 H. unfold nth_gen, nth_space in *.
         simpl. destruct (Nat.eq_dec gen to).
         -- subst gen. rewrite cvmgil_eq; simpl; assumption.
         -- rewrite cvmgil_not_eq; assumption.
-      * assert (0 <= Z.of_nat gen < Zlength (spaces (ti_heap t_info))). {
+      * assert (0 <= Z.of_nat gen < Zlength (spaces h)). {
           split. 1: apply Nat2Z.is_nonneg. rewrite Zlength_correct.
           apply inj_lt. red in H4. lia. }
         rewrite <- (Nat2Z.id gen) at 3. rewrite nth_Znth.
@@ -3021,15 +3009,15 @@ Proof.
 Qed.
 
 Lemma lcv_super_compatible_unchanged: forall
-    g t_info roots outlier to v
-    (Hi : 0 <= Z.of_nat to < Zlength (spaces (ti_heap t_info)))
-    (Hh : has_space (Znth (Z.of_nat to) (spaces (ti_heap t_info))) (vertex_size g v)),
+    g h frames roots outlier to v
+    (Hi : 0 <= Z.of_nat to < Zlength (spaces h))
+    (Hh : has_space (Znth (Z.of_nat to) (spaces h)) (vertex_size g v)),
     graph_has_gen g to -> graph_has_v g v ->
-    super_compatible (g, t_info, roots) outlier ->
-    super_compatible
-      (lgraph_copy_v g v to,
-       (cut_thread_info t_info (Z.of_nat to) (vertex_size g v) Hi Hh),
-       roots) outlier.
+    super_compatible' g h frames roots outlier ->
+    super_compatible'
+      (lgraph_copy_v g v to)
+       (cut_heap h (Z.of_nat to) (vertex_size g v) Hi Hh)
+       frames roots outlier.
 Proof.
   intros. destruct H1 as [? [? [? ?]]]. split; [|split; [|split]].
   - apply lcv_graph_thread_info_compatible; assumption.
@@ -3039,20 +3027,19 @@ Proof.
 Qed.
 
 Lemma lcv_super_compatible: forall
-    g t_info roots outlier to v z
-    (Hi : 0 <= Z.of_nat to < Zlength (spaces (ti_heap t_info)))
-    (Hh : has_space (Znth (Z.of_nat to) (spaces (ti_heap t_info))) (vertex_size g v))
+    g h frames roots outlier to v z
+    (Hi : 0 <= Z.of_nat to < Zlength (spaces h))
+    (Hh : has_space (Znth (Z.of_nat to) (spaces h)) (vertex_size g v))
     (Hm : 0 <= z < Zlength roots),
     graph_has_gen g to -> graph_has_v g v ->
-    super_compatible (g, t_info, roots) outlier ->
-    super_compatible
-      (lgraph_copy_v g v to,
-       update_thread_info_frames
-         (cut_thread_info t_info (Z.of_nat to) (vertex_size g v) Hi Hh)
-         (update_frames (ti_frames t_info)
-           (upd_Znth z (frames2roots (ti_frames t_info))
-              (vertex_address g (new_copied_v g to)))),
-       upd_Znth z roots (inr (new_copied_v g to))) outlier.
+    super_compatible' g h frames roots outlier ->
+    super_compatible'
+      (lgraph_copy_v g v to)
+      (cut_heap h (Z.of_nat to) (vertex_size g v) Hi Hh)
+      (update_frames frames
+           (upd_Znth z (frames2roots frames)
+              (vertex_address g (new_copied_v g to))))
+      (upd_Znth z roots (inr (new_copied_v g to))) outlier.
 Proof.
   intros. destruct H1 as [? [? [? ?]]]. split; [|split; [|split]].
   - apply lcv_graph_thread_info_compatible; assumption.
@@ -3082,76 +3069,71 @@ Lemma utia_ti_heap: forall t_info i ad (Hm : 0 <= i < MAX_ARGS),
     ti_heap (update_thread_info_arg t_info i ad Hm) = ti_heap t_info.
 Proof. intros. simpl. reflexivity. Qed.
 
-Lemma cti_space_not_eq: forall t_info i s n
-    (Hi : 0 <= i < Zlength (spaces (ti_heap t_info)))
-    (Hh : has_space (Znth i (spaces (ti_heap t_info))) s),
+Lemma cti_space_not_eq: forall h i s n
+    (Hi : 0 <= i < Zlength (spaces h))
+    (Hh : has_space (Znth i (spaces h)) s),
     (Z.of_nat n) <> i ->
-    nth_space (cut_thread_info t_info i s Hi Hh) n = nth_space t_info n.
+    nth_space (cut_heap h i s Hi Hh) n = nth_space h n.
 Proof.
   intros. rewrite !nth_space_Znth. simpl.
   pose proof (Nat2Z.is_nonneg n). remember (Z.of_nat n). clear Heqz.
-  remember (spaces (ti_heap t_info)). destruct (Z_lt_le_dec z (Zlength l)).
+  remember (spaces h). destruct (Z_lt_le_dec z (Zlength l)).
   - assert (0 <= z < Zlength l) by lia.
     rewrite upd_Znth_diff; [reflexivity |assumption..].
   - rewrite !Znth_overflow;
       [reflexivity | | rewrite upd_Znth_Zlength by assumption]; lia.
 Qed.
 
-Lemma cti_space_eq: forall t_info i s
-    (Hi : 0 <= Z.of_nat i < Zlength (spaces (ti_heap t_info)))
-    (Hh : has_space (Znth (Z.of_nat i) (spaces (ti_heap t_info))) s),
-    nth_space (cut_thread_info t_info (Z.of_nat i) s Hi Hh) i =
-    cut_space (Znth (Z.of_nat i) (spaces (ti_heap t_info))) s Hh.
+Lemma cti_space_eq: forall h i s
+    (Hi : 0 <= Z.of_nat i < Zlength (spaces h))
+    (Hh : has_space (Znth (Z.of_nat i) (spaces h)) s),
+    nth_space (cut_heap h (Z.of_nat i) s Hi Hh) i =
+    cut_space (Znth (Z.of_nat i) (spaces h)) s Hh.
 Proof.
   intros. rewrite nth_space_Znth. simpl. rewrite upd_Znth_same by assumption.
   reflexivity.
 Qed.
 
-Lemma cti_gen_size: forall t_info i s n
-    (Hi : 0 <= i < Zlength (spaces (ti_heap t_info)))
-    (Hh : has_space (Znth i (spaces (ti_heap t_info))) s),
-    gen_size (cut_thread_info t_info i s Hi Hh) n =
-    gen_size t_info n.
+Lemma cti_gen_size: forall h i s n
+    (Hi : 0 <= i < Zlength (spaces h))
+    (Hh : has_space (Znth i (spaces h)) s),
+    gen_size (cut_heap h i s Hi Hh) n =
+    gen_size h n.
 Proof.
   intros. unfold gen_size. destruct (Z.eq_dec (Z.of_nat n) i).
   - subst i. rewrite cti_space_eq. simpl. rewrite nth_space_Znth. reflexivity.
   - rewrite cti_space_not_eq; [reflexivity | assumption].
 Qed.
 
-Lemma cti_space_start: forall t_info i s  n
-    (Hi : 0 <= i < Zlength (spaces (ti_heap t_info)))
-    (Hh : has_space (Znth i (spaces (ti_heap t_info))) s),
-    space_start (nth_space (cut_thread_info t_info i s Hi Hh) n) =
-    space_start (nth_space t_info n).
+Lemma cti_space_start: forall h i s  n
+    (Hi : 0 <= i < Zlength (spaces h))
+    (Hh : has_space (Znth i (spaces h)) s),
+    space_start (nth_space (cut_heap h i s Hi Hh) n) =
+    space_start (nth_space h n).
 Proof.
   intros. destruct (Z.eq_dec (Z.of_nat n) i).
   - subst i. rewrite cti_space_eq. simpl. rewrite nth_space_Znth. reflexivity.
   - rewrite cti_space_not_eq; [reflexivity | assumption].
 Qed.
 
-Lemma utiacti_gen_size: forall t_info i1 s fr n
-    (Hi : 0 <= i1 < Zlength (spaces (ti_heap t_info)))
-    (Hh : has_space (Znth i1 (spaces (ti_heap t_info))) s),
-    gen_size 
-       (update_thread_info_frames 
-              (cut_thread_info t_info i1 s Hi Hh) fr)
-                         n =
-    gen_size t_info n.
+Lemma utiacti_gen_size: forall h i1 s n
+    (Hi : 0 <= i1 < Zlength (spaces h))
+    (Hh : has_space (Znth i1 (spaces h)) s),
+    gen_size (cut_heap h i1 s Hi Hh) n =
+    gen_size h n.
 Proof.
   intros. unfold gen_size, nth_space. simpl.  apply cti_gen_size with (Hi:=Hi).
 Qed.
 
-Lemma utiacti_space_start: forall t_info i1 s fr n
-    (Hi : 0 <= i1 < Zlength (spaces (ti_heap t_info)))
-    (Hh : has_space (Znth i1 (spaces (ti_heap t_info))) s),
-    space_start
-      (nth_space (update_thread_info_frames (cut_thread_info t_info i1 s Hi Hh) fr)
-                 n) = space_start (nth_space t_info n).
+Lemma utiacti_space_start: forall h i1 s n
+    (Hi : 0 <= i1 < Zlength (spaces h))
+    (Hh : has_space (Znth i1 (spaces h)) s),
+    space_start (nth_space (cut_heap h i1 s Hi Hh) n) = space_start (nth_space h n).
 Proof. intros. unfold nth_space.  apply cti_space_start. Qed.
 
 Definition thread_info_relation t t':=
-  ti_heap_p t = ti_heap_p t' /\ (forall n, gen_size t n = gen_size t' n) /\
-  forall n, space_start (nth_space t n) = space_start (nth_space t' n).
+  ti_heap_p t = ti_heap_p t' /\ (forall n, gen_size t.(ti_heap) n = gen_size t'.(ti_heap) n) /\
+  forall n, space_start (nth_space t.(ti_heap) n) = space_start (nth_space t'.(ti_heap) n).
 
 Lemma tir_id: forall t, thread_info_relation t t.
 Proof. intros. red. split; [|split]; reflexivity. Qed.
@@ -3373,9 +3355,9 @@ Lemma lgd_roots_compatible: forall g outlier roots e v,
 Proof. intros. destruct H. split; [|apply lgd_rgc]; assumption. Qed.
 
 Lemma lgd_graph_thread_info_compatible:
-  forall (g : LGraph) (t_info : thread_info) e (v' : VType),
-  graph_thread_info_compatible g t_info ->
-  graph_thread_info_compatible (labeledgraph_gen_dst g e v') t_info.
+  forall (g : LGraph) (h : heap) e (v' : VType),
+  graph_heap_compatible g h ->
+  graph_heap_compatible (labeledgraph_gen_dst g e v') h.
 Proof.
   intros; destruct H; split; assumption. Qed.
 
@@ -4061,8 +4043,8 @@ Definition do_generation_relation (from to: nat)
     do_scan_relation from to (number_of_vertices (nth_gen g to)) g1 g2 /\
     g' = reset_graph from g2.
 
-Definition space_address (t_info: thread_info) (gen: nat) :=
-  offset_val (SPACE_STRUCT_SIZE * Z.of_nat gen) (ti_heap_p t_info).
+Definition space_address (heap_p: val) (gen: nat) :=
+  offset_val (SPACE_STRUCT_SIZE * Z.of_nat gen) heap_p.
 
 Definition enough_space_to_have_g g t_info from to: Prop :=
   graph_gen_size g from <= rest_gen_size t_info to.
@@ -4155,10 +4137,10 @@ Proof.
   rewrite remove_ve_vlabel_unchanged. reflexivity.
 Qed.
 
-Lemma graph_thread_info_compatible_reset: forall g t_info gen,
-    graph_thread_info_compatible g t_info ->
-    graph_thread_info_compatible (reset_graph gen g)
-                                 (reset_nth_heap_thread_info gen t_info).
+Lemma graph_thread_info_compatible_reset: forall g h gen,
+    graph_heap_compatible g h ->
+    graph_heap_compatible (reset_graph gen g)
+                                 (reset_nth_heap gen h).
 Proof.
   intros. destruct H as [? [? ?]].
   split; [|split]; [|simpl; rewrite reset_nth_gen_info_length..].
@@ -4174,51 +4156,16 @@ Proof.
       destruct H as [? [? ?]]. split. 1: assumption. split. 1: assumption.
       rewrite pvs_reset_unchanged. assumption.
   - rewrite remove_ve_glabel_unchanged.
-    destruct (le_lt_dec (length (spaces (ti_heap t_info))) gen).
+    destruct (le_lt_dec (length (spaces h)) gen).
     + rewrite reset_nth_space_overflow; assumption.
     + rewrite reset_nth_space_Znth by assumption. rewrite <- upd_Znth_map. simpl.
-      remember (spaces (ti_heap t_info)).
+      remember (spaces h).
       assert (0 <= Z.of_nat gen < Zlength l0) by (rewrite Zlength_correct; lia).
       replace (space_start (Znth (Z.of_nat gen) l0))
         with (Znth (Z.of_nat gen) (map space_start l0)) by (rewrite Znth_map; auto).
       rewrite upd_Znth_unchanged; [|rewrite Zlength_map]; assumption.
   - rewrite remove_ve_glabel_unchanged, reset_nth_space_length. assumption.
 Qed.
-
-(*
-Lemma upd_bunch_rf_compatible: forall f_info roots z r,
-    roots_fi_compatible roots f_info ->
-    roots_fi_compatible (upd_bunch z f_info roots r) f_info.
-Proof.
-  intros. unfold roots_fi_compatible in *. destruct H.
-  assert (Zlength (upd_bunch z f_info roots r) = Zlength (live_roots_indices f_info))
-    by (rewrite upd_bunch_Zlength; assumption). split; intros. 1: assumption.
-  rewrite H1 in *. rewrite <- H in *.
-  destruct (Z.eq_dec (Znth i (live_roots_indices f_info))
-                     (Znth z (live_roots_indices f_info))).
-  - rewrite !upd_bunch_same; try assumption; try reflexivity.
-    rewrite H4 in e; assumption.
-  - rewrite !upd_bunch_diff; try assumption; [apply H0 | rewrite <- H4]; assumption.
-Qed.
-
-Lemma upd_roots_rf_compatible: forall from to roots t_info p g,
-    roots_ti_compatible roots tnfo ->
-    roots_fi_compatible (upd_roots from to p g roots) t_info.
-Proof.
-  intros. unfold upd_roots. destruct p; [|assumption]. destruct (Znth z roots).
-  1: destruct s; assumption. if_tac. 2: assumption.
-  destruct (raw_mark (vlabel g v)); apply upd_bunch_rf_compatible; assumption.
-Qed.
-*)
-
-(*
-Definition np_roots_rel from f_info (roots roots': roots_t) (l: list Z) : Prop :=
-  let lri := live_roots_indices f_info in
-  let maped_lri := (map (flip Znth lri) l) in
-  forall v j, Znth j roots' = inr v ->
-              (In (Znth j lri) maped_lri -> vgeneration v <> from) /\
-              (~ In (Znth j lri) maped_lri -> Znth j roots = inr v).
-*)
 
 Definition np_roots_rel from (roots roots': roots_t) (l: list Z) : Prop :=
   forall v j, 
@@ -4504,11 +4451,10 @@ Proof.
   rewrite graph_has_v_reset in H0. destruct H0. assumption.
 Qed.
 
-Lemma super_compatible_reset: forall g t_info roots outlier gen,
+Lemma super_compatible_reset: forall g h frames roots outlier gen,
     roots_have_no_gen roots gen ->
-    super_compatible (g, t_info, roots) outlier ->
-    super_compatible (reset_graph gen g,
-                      reset_nth_heap_thread_info gen t_info, roots) outlier.
+    super_compatible' g h frames roots outlier ->
+    super_compatible' (reset_graph gen g) (reset_nth_heap gen h) frames roots outlier.
 Proof.
   intros. destruct H0 as [? [? [? ?]]]. split; [|split; [|split]].
   - apply graph_thread_info_compatible_reset; assumption.
@@ -4691,13 +4637,13 @@ Definition gen_v_num (g: LGraph) (gen: nat): nat := number_of_vertices (nth_gen 
 
 Definition nth_gen_size (n: nat) := NURSERY_SIZE * two_p (Z.of_nat n).
 
-Definition nth_gen_size_spec (tinfo: thread_info) (n: nat): Prop :=
-  if Val.eq (nth_space tinfo n).(space_start) nullval
+Definition nth_gen_size_spec (h: heap) (n: nat): Prop :=
+  if Val.eq (nth_space h n).(space_start) nullval
   then True
-  else gen_size tinfo n = nth_gen_size n.
+  else gen_size h n = nth_gen_size n.
 
-Definition ti_size_spec (tinfo: thread_info): Prop :=
-  Forall (nth_gen_size_spec tinfo) (nat_inc_list (Z.to_nat MAX_SPACES)).
+Definition ti_size_spec (h: heap): Prop :=
+  Forall (nth_gen_size_spec h) (nat_inc_list (Z.to_nat MAX_SPACES)).
 
 Definition safe_to_copy_gen g from to: Prop :=
   nth_gen_size from <= nth_gen_size to - graph_gen_size g to.
@@ -4740,22 +4686,22 @@ Proof.
   reflexivity.
 Qed.
 
-Lemma space_start_isptr: forall (g: LGraph) (t_info: thread_info) i,
-    graph_thread_info_compatible g t_info ->
-    0 <= i < Zlength (spaces (ti_heap t_info)) ->
+Lemma space_start_isptr: forall (g: LGraph) (h: heap) i,
+    graph_heap_compatible g h ->
+    0 <= i < Zlength (spaces h) ->
     graph_has_gen g (Z.to_nat i) ->
-    isptr (space_start (Znth i (spaces (ti_heap t_info)))).
+    isptr (space_start (Znth i (spaces h))).
 Proof.
   intros. destruct (gt_gs_compatible _ _ H _ H1) as [? _].
   rewrite nth_space_Znth in H2. rewrite Z2Nat.id in H2 by lia. rewrite <- H2.
   apply start_isptr.
 Qed.
 
-Lemma space_start_isnull: forall (g: LGraph) (t_info: thread_info) i,
-    graph_thread_info_compatible g t_info ->
-    0 <= i < Zlength (spaces (ti_heap t_info)) ->
+Lemma space_start_isnull: forall (g: LGraph) (h: heap) i,
+    graph_heap_compatible g h ->
+    0 <= i < Zlength (spaces h) ->
     ~ graph_has_gen g (Z.to_nat i) ->
-    space_start (Znth i (spaces (ti_heap t_info))) = nullval.
+    space_start (Znth i (spaces h)) = nullval.
 Proof.
   intros. unfold graph_has_gen in H1. destruct H as [_ [? ?]].
   rewrite Forall_forall in H. symmetry. apply H. rewrite <- map_skipn.
@@ -4769,23 +4715,23 @@ Proof.
   rewrite (Z.max_r 0 (Zlength l)) by rep_lia. rewrite Z.max_r; rep_lia.
 Qed.
 
-Lemma space_start_is_pointer_or_null: forall (g: LGraph) (t_info: thread_info) i,
-    graph_thread_info_compatible g t_info ->
-    0 <= i < Zlength (spaces (ti_heap t_info)) ->
-    is_pointer_or_null (space_start (Znth i (spaces (ti_heap t_info)))).
+Lemma space_start_is_pointer_or_null: forall (g: LGraph) (h: heap) i,
+    graph_heap_compatible g h ->
+    0 <= i < Zlength (spaces h) ->
+    is_pointer_or_null (space_start (Znth i (spaces h))).
 Proof.
   intros. destruct (graph_has_gen_dec g (Z.to_nat i)).
   - apply val_lemmas.isptr_is_pointer_or_null. eapply space_start_isptr; eauto.
-  - cut (space_start (Znth i (spaces (ti_heap t_info))) = nullval).
+  - cut (space_start (Znth i (spaces h)) = nullval).
     + intros. rewrite H1. apply mapsto_memory_block.is_pointer_or_null_nullval.
     + eapply space_start_isnull; eauto.
 Qed.
 
-Lemma space_start_isptr_iff: forall (g: LGraph) (t_info: thread_info) i,
-    graph_thread_info_compatible g t_info ->
-    0 <= i < Zlength (spaces (ti_heap t_info)) ->
+Lemma space_start_isptr_iff: forall (g: LGraph) (h: heap) i,
+    graph_heap_compatible g h ->
+    0 <= i < Zlength (spaces h) ->
     graph_has_gen g (Z.to_nat i) <->
-    isptr (space_start (Znth i (spaces (ti_heap t_info)))).
+    isptr (space_start (Znth i (spaces h))).
 Proof.
   intros. split; intros.
   - eapply space_start_isptr; eauto.
@@ -4793,37 +4739,37 @@ Proof.
     eapply space_start_isnull in n; eauto. rewrite n in H1. inversion H1.
 Qed.
 
-Lemma space_start_isnull_iff: forall (g: LGraph) (t_info: thread_info) i,
-    graph_thread_info_compatible g t_info ->
-    0 <= i < Zlength (spaces (ti_heap t_info)) ->
+Lemma space_start_isnull_iff: forall (g: LGraph) (h: heap) i,
+    graph_heap_compatible g h ->
+    0 <= i < Zlength (spaces h) ->
     ~ graph_has_gen g (Z.to_nat i) <->
-    space_start (Znth i (spaces (ti_heap t_info))) = nullval.
+    space_start (Znth i (spaces h)) = nullval.
 Proof.
   intros. split; intros. 1: eapply space_start_isnull; eauto.
   destruct (graph_has_gen_dec g (Z.to_nat i)). 2: assumption. exfalso.
   eapply space_start_isptr in g0; eauto. rewrite H1 in g0. inversion g0.
 Qed.
 
-Lemma ti_size_gen: forall (g : LGraph) (t_info : thread_info) (gen : nat),
-    graph_thread_info_compatible g t_info ->
-    graph_has_gen g gen -> ti_size_spec t_info ->
-    gen_size t_info gen = nth_gen_size gen.
+Lemma ti_size_gen: forall (g : LGraph) (h : heap) (gen : nat),
+    graph_heap_compatible g h ->
+    graph_has_gen g gen -> ti_size_spec h ->
+    gen_size h gen = nth_gen_size gen.
 Proof.
   intros. red in H1. rewrite Forall_forall in H1.
-  assert (0 <= (Z.of_nat gen) < Zlength (spaces (ti_heap t_info))). {
+  assert (0 <= (Z.of_nat gen) < Zlength (spaces h)). {
     split. 1: rep_lia. rewrite Zlength_correct. apply inj_lt.
     destruct H as [_ [_ ?]]. red in H0. lia. }
-  assert (nth_gen_size_spec t_info gen). {
+  assert (nth_gen_size_spec h gen). {
     apply H1. rewrite nat_inc_list_In_iff. destruct H as [_ [_ ?]]. red in H0.
-    rewrite <- (spaces_size (ti_heap t_info)), ZtoNat_Zlength. lia. } red in H3.
-  destruct (Val.eq (space_start (nth_space t_info gen)) nullval). 2: assumption.
+    rewrite <- (spaces_size h), ZtoNat_Zlength. lia. } red in H3.
+  destruct (Val.eq (space_start (nth_space h gen)) nullval). 2: assumption.
   rewrite nth_space_Znth in e. erewrite <- space_start_isnull_iff in e; eauto.
   unfold graph_has_gen in e. exfalso; apply e. rewrite Nat2Z.id. assumption.
 Qed.
 
-Lemma ti_size_gt_0: forall (g : LGraph) (t_info : thread_info) (gen : nat),
-    graph_thread_info_compatible g t_info ->
-    graph_has_gen g gen -> ti_size_spec t_info -> 0 < gen_size t_info gen.
+Lemma ti_size_gt_0: forall (g : LGraph) (h : heap) (gen : nat),
+    graph_heap_compatible g h ->
+    graph_has_gen g gen -> ti_size_spec h -> 0 < gen_size h gen.
 Proof.
   intros. erewrite ti_size_gen; eauto. unfold nth_gen_size. apply Z.mul_pos_pos.
   - rewrite NURSERY_SIZE_eq. vm_compute. reflexivity.
@@ -5445,10 +5391,9 @@ Definition garbage_collect_relation
   exists n, garbage_collect_loop (nat_inc_list (S n)) roots1 g1 roots2 g2 /\
             safe_to_copy_gen g2 n (S n).
 
-Definition garbage_collect_condition (g: LGraph) (t_info : thread_info)
+Definition garbage_collect_condition (g: LGraph) (h : heap)
            (roots : roots_t) : Prop :=
-  graph_unmarked g /\ no_backward_edge g /\ no_dangling_dst g /\
-  ti_size_spec t_info.
+  graph_unmarked g /\ no_backward_edge g /\ no_dangling_dst g /\ ti_size_spec h.
 
 Local Open Scope Z_scope.
 
@@ -5478,8 +5423,8 @@ Proof.
 Qed.
 
 Lemma ans_nth_old: forall ti sp i (Hs: 0 <= i < MAX_SPACES) gen,
-    gen <> Z.to_nat i -> nth_space (ti_add_new_space ti sp i Hs) gen =
-                         nth_space ti gen.
+    gen <> Z.to_nat i -> nth_space (ti_add_new_space ti sp i Hs).(ti_heap) gen =
+                         nth_space ti.(ti_heap) gen.
 Proof.
   intros. rewrite !nth_space_Znth. simpl. rewrite upd_Znth_diff_strong.
   - reflexivity.
@@ -5488,7 +5433,7 @@ Proof.
 Qed.
 
 Lemma ans_nth_new: forall ti sp i (Hs: 0 <= i < MAX_SPACES),
-    nth_space (ti_add_new_space ti sp i Hs) (Z.to_nat i) = sp.
+    nth_space (ti_add_new_space ti sp i Hs).(ti_heap) (Z.to_nat i) = sp.
 Proof.
   intros. rewrite nth_space_Znth. simpl. rewrite Z2Nat.id by lia.
   rewrite upd_Znth_same; [reflexivity | rewrite spaces_size; assumption].
@@ -5502,13 +5447,13 @@ Proof.
 Qed.
 
 Lemma gti_compatible_add: forall g ti gi sp i (Hs: 0 <= i < MAX_SPACES),
-    graph_thread_info_compatible g ti ->
+    graph_heap_compatible g ti.(ti_heap) ->
     ~ graph_has_gen g (Z.to_nat i) -> graph_has_gen g (Z.to_nat (i - 1)) ->
     (forall (gr: LGraph), generation_space_compatible gr (Z.to_nat i, gi, sp)) ->
-    graph_thread_info_compatible (lgraph_add_new_gen g gi)
-                                 (ti_add_new_space ti sp i Hs).
+    graph_heap_compatible (lgraph_add_new_gen g gi)
+                                 (ti_add_new_space ti sp i Hs).(ti_heap).
 Proof.
-  intros. unfold graph_thread_info_compatible in *. destruct H as [? [? ?]].
+  intros. unfold graph_heap_compatible in *. destruct H as [? [? ?]].
   assert (length (g_gen (glabel g)) = Z.to_nat i). {
     clear -H0 H1. unfold graph_has_gen in *.
     rewrite Z2Nat.inj_sub in H1 by lia. simpl in H1. lia. }
@@ -5610,8 +5555,8 @@ Proof.
 Qed.
 
 Lemma ti_size_spec_add: forall ti sp i (Hs: 0 <= i < MAX_SPACES),
-    total_space sp = nth_gen_size (Z.to_nat i) -> ti_size_spec ti ->
-    ti_size_spec (ti_add_new_space ti sp i Hs).
+    total_space sp = nth_gen_size (Z.to_nat i) -> ti_size_spec ti.(ti_heap) ->
+    ti_size_spec (ti_add_new_space ti sp i Hs).(ti_heap).
 Proof.
   intros. unfold ti_size_spec in *. rewrite Forall_forall in *. intros.
   specialize (H0 _ H1). unfold nth_gen_size_spec in *.
@@ -5628,10 +5573,12 @@ Proof.
   rewrite ang_nth_old; auto. unfold graph_has_gen in *. lia.
 Qed.
 
-Lemma ans_space_address: forall ti sp i (Hs: 0 <= i < MAX_SPACES) j,
-    space_address (ti_add_new_space ti sp i Hs) (Z.to_nat j) =
-    space_address ti (Z.to_nat j).
+(*
+Lemma ans_space_address: forall h heap_p sp i (Hs: 0 <= i < MAX_SPACES) j,
+    space_address heap_p (add_new_space h sp i Hs) (Z.to_nat j) =
+    space_address heap_p (Z.to_nat j).
 Proof. intros. unfold space_address. simpl. reflexivity. Qed.
+*)
 
 Lemma ang_make_header: forall g gi v,
     make_header g v = make_header (lgraph_add_new_gen g gi) v.
@@ -5717,9 +5664,9 @@ Qed.
 
 Lemma gcc_add: forall g ti gi sp i (Hs: 0 <= i < MAX_SPACES) roots,
     number_of_vertices gi = O -> total_space sp = nth_gen_size (Z.to_nat i) ->
-    garbage_collect_condition g ti roots ->
+    garbage_collect_condition g ti.(ti_heap) roots ->
     garbage_collect_condition (lgraph_add_new_gen g gi)
-                              (ti_add_new_space ti sp i Hs) roots.
+                              (ti_add_new_space ti sp i Hs).(ti_heap) roots.
 Proof.
   intros. destruct H1 as [? [? [? ?]]]. split; [|split; [|split]].
   - apply graph_unmarked_add; assumption.
@@ -5736,12 +5683,12 @@ Proof.
   cut (two_p (16 + Z.of_nat i) > 0); [|apply two_p_gt_ZERO]; lia.
 Qed.
 
-Lemma gc_cond_implies_do_gen_cons: forall g t_info roots i,
+Lemma gc_cond_implies_do_gen_cons: forall g h roots i,
     safe_to_copy_to_except g i ->
     graph_has_gen g (S i) ->
-    graph_thread_info_compatible g t_info ->
-    garbage_collect_condition g t_info roots ->
-    do_generation_condition g t_info (*roots*) i (S i).
+    graph_heap_compatible g h ->
+    garbage_collect_condition g h roots ->
+    do_generation_condition g h i (S i).
 Proof.
   intros. destruct H2 as [? [? [? ?]]].
   assert (graph_has_gen g i) by (unfold graph_has_gen in H0 |-*; lia).
@@ -5751,16 +5698,15 @@ Proof.
     destruct (gt_gs_compatible _ _ H1 _ H0) as [_ [_ ?]].
     destruct (gt_gs_compatible _ _ H1 _ H6) as [_ [_ ?]].
     fold (graph_gen_size g (S i)) in H7. fold (graph_gen_size g i) in H8.
-    rewrite <- H7. fold (gen_size t_info (S i)).
-    destruct (space_order (nth_space t_info i)) as [_ ?].
-    fold (gen_size t_info i) in H9. rewrite <- H8 in H9.
-    transitivity (gen_size t_info i). 1: assumption.
+    rewrite <- H7. fold (gen_size h (S i)).
+    destruct (space_order (nth_space h i)) as [_ ?].
+    fold (gen_size h i) in H9. rewrite <- H8 in H9.
+    transitivity (gen_size h i). 1: assumption.
     rewrite (ti_size_gen _ _ _ H1 H6 H5), (ti_size_gen _ _ _ H1 H0 H5).
     apply H; [lia.. | assumption].
   - apply graph_unmarked_copy_compatible; assumption.
   - rewrite (ti_size_gen _ _ _ H1 H0 H5). apply ngs_0_lt.
   - rewrite graph_gen_unmarked_iff in H2. apply H2.
-(*  - red.*)
 Qed.
 
 Lemma do_gen_no_dangling_dst: forall g1 g2 roots1 roots2 from to,
@@ -5877,7 +5823,7 @@ Qed.
 
 Lemma ti_relation_size_spec: forall t_info1 t_info2 : thread_info,
     thread_info_relation t_info1 t_info2 ->
-    ti_size_spec t_info1 -> ti_size_spec t_info2.
+    ti_size_spec t_info1.(ti_heap) -> ti_size_spec t_info2.(ti_heap).
 Proof.
   intros. unfold ti_size_spec in *. rewrite Forall_forall in *. intros.
   specialize (H0 _ H1). unfold nth_gen_size_spec in *. destruct H as [? [? ?]].
@@ -5888,16 +5834,15 @@ Lemma do_gen_gcc: forall g1 t_info1 roots1 g2 t_info2 roots2 i out,
     super_compatible (g1, t_info1, roots1) out ->
     firstn_gen_clear g1 i -> graph_has_gen g1 (S i) ->
     thread_info_relation t_info1 t_info2 ->
-    garbage_collect_condition g1 t_info1 roots1 ->
+    garbage_collect_condition g1 t_info1.(ti_heap) roots1 ->
     do_generation_relation i (S i) roots1 roots2 g1 g2 ->
-    garbage_collect_condition g2 t_info2 roots2.
+    garbage_collect_condition g2 t_info2.(ti_heap) roots2.
 Proof.
   intros. destruct H3 as [? [? [? ?]]].
   assert (gen_unmarked g1 (S i)) by (rewrite graph_gen_unmarked_iff in H3; apply H3).
   assert (no_dangling_dst g2). {
     eapply do_gen_no_dangling_dst; eauto.
     - apply graph_unmarked_copy_compatible; assumption.
-(*    - apply (proj1 H7).*)
     - destruct H as [_ [_ [[_ ?] _]]]. assumption. }
   split; [|split; [|split]]; auto.
   - eapply do_gen_graph_unmarked; eauto.
